src/lowparse/LowParse.SteelST.Recursive.fst
@@ -665,13 +665,6 @@ let jump_recursive
   noop ();
   return res
 
-let get_children
-  (#p: parse_recursive_param)
-  (s: serialize_recursive_param p)
-  (x: p.t)
-: Tot (list p.t)
-= dsnd (s.synth_recip x)
-
 module LPC = LowParse.SteelST.Combinators
 module NL = LowParse.SteelST.VCList
 
@@ -795,29 +788,6 @@ let elim_recursive_as_nlist
   ar
 
 #pop-options
-
-[@@erasable]
-noeq
-type fold_recursive_t
-  (#p: parse_recursive_param)
-  (s: serialize_recursive_param p)
-  (t: Type)
-: Type
-= {
-    step: (t -> p.t -> t);
-    fold: (t -> p.t -> t);
-    prf: (
-      (init: t) ->
-      (x: p.t) ->
-      Lemma
-      (fold init x ==
-        List.Tot.fold_left
-          fold
-          (step init x)
-          (get_children s x) 
-      )
-    );
-  }
 
 let fold_recursive_restore_t
   (p: parse_recursive_param)
@@ -1035,33 +1005,6 @@ let seq_append_injective
   assert (sr1 `Seq.equal` Seq.slice s (Seq.length s - Seq.length sr1) (Seq.length s));
   Seq.lemma_split s (Seq.length sl1);
   Seq.lemma_split s (Seq.length s - Seq.length sr1)
-
-let list_fold_left_append
-  (#a #b: Type)
-  (f: a -> b -> Tot a)
-  (l1 l2: list b)
-  (x: a)
-: Tot (squash (List.Tot.fold_left f x (l1 `List.Tot.append` l2) == List.Tot.fold_left f (List.Tot.fold_left f x l1) l2))
-= List.Tot.fold_left_append f l1 l2
-
-let fold_recursive_cons_eq
-  (#p: parse_recursive_param)
-  (s: serialize_recursive_param p)
-  (#t: Type)
-  (fold: fold_recursive_t s t)
-  (init: t)
-  (hd: p.t)
-  (tl: list p.t)
-  (l': list p.t)
-: Lemma
-  (requires (
-    l' == List.Tot.append (get_children s hd) tl
-  ))
-  (ensures (
-    List.Tot.fold_left fold.fold init (hd :: tl) == List.Tot.fold_left fold.fold (fold.step init hd) l'
-  ))
-= fold.prf init hd;
-  list_fold_left_append fold.fold (get_children s hd) tl (fold.step init hd)
 
 let get_children_synth
   (#p: parse_recursive_param)
@@ -1353,38 +1296,6 @@ let fold_recursive
   let _ = NL.elim_nlist_one (parse_recursive p) (SZ.v n0) a0 in
   vpattern_rewrite (aparse _ a0) _;
   vpattern_rewrite state _
-
-[@@erasable]
-noeq
-type pred_recursive_t
-  (#p: parse_recursive_param)
-  (s: serialize_recursive_param p)
-: Type
-= {
-    base: (p.t -> bool);
-    pred: (p.t -> bool);
-    prf: (
-      (x: p.t) ->
-      Lemma
-      (pred x == (base x && List.Tot.for_all pred (get_children s x)))
-    );
-  }
-
-let fold_of_pred_recursive
-  (#p: parse_recursive_param)
-  (s: serialize_recursive_param p)
-  (pred: pred_recursive_t s)
-: Tot (fold_recursive_t s bool)
-= let base = pred.base in
-  let pr = pred.pred in
-  {
-    step = LowParse.WellFounded.forall_list_f_weak base;
-    fold = LowParse.WellFounded.forall_list_f_weak pr;
-    prf = (fun aux x ->
-      pred.prf x;
-      LowParse.WellFounded.for_all_fold_left_aux pr (aux && base x) (get_children s x)
-    );
-  }
 
 inline_for_extraction
 let pred_recursive_base_t
